# Exercise set 6.3

  

![](https://cdn.mathpix.com/cropped/2023_12_27_9af192d7c8a1ca8a8e27g-1.jpg?height=294&width=320&top_left_y=270&top_left_x=251)

  

$(A \cap B) \cup C$

  

![](https://cdn.mathpix.com/cropped/2023_12_27_9af192d7c8a1ca8a8e27g-1.jpg?height=294&width=306&top_left_y=270&top_left_x=635)

  

$A \cap(B \cup C)$

  

Using the venn diagrams, you can see that, $(A \cap B) \cup C \neq A \cap(B \cup C)$

  

Let $A:\{x\}, B=\{y\}, C=\{x, z\}$

  

$A \notin B$ and $B \nsubseteq C$, however $A \leq C$

  

$A-(B-C)=(A-B)-C \quad($ false $)$

  

Let $A=[1,2,3,4], B=\{3,4,5,6], C=\{4,5,6,7]$

  

$A \quad-(B-C) \quad(A-B)-C$

  

$\{1,2,3,4]-[3]=\{1,2,4] \quad\{1,2\}-[4,5,6,9]=[1,2]$

  

$$

\{1,2,4] \neq[1,2]

$$

  

$$

\therefore A-(B-C) \neq(A-B)-C

$$

  

$A \cap(A \cup B): A \quad$ (True)

  

if $x$ is in $A \cap(A \cup B)$ then $x$ is in $A$ and $A \cup B$

  

if $x$ is in $B$ it also satisfies the condition because $x$ is in $A$ also

  

Therefore any element in $x$ in $A \cap(A \cup B)$ must be in $A$ and we can say that $A \cap(A \cup B) \leq A$

  

if $y$ is in $A$, then it satisfies the condition $y \in A \cap(A \cup B)$ because $y$ in both $A$ and $A \cup B$ Therefore, $A \leq A \cap(A \cup B)$

  

Since $A \cap(A \cup B) \subseteq A$ and $A \subseteq A \cap(A \cup B), A \cap(A \cup B)=A$

  

if $A \leq C$ and $B \leq C$ then $A \cup B \leq C$ (Tnue)

  

if $A \subseteq C$ and $B \subseteq C$, it means that every element of $A$ is an element of $C$, and every element of $B$ is abso an element of $C$. Every element in $A \cup B$ must be in either $A$ or $B$ or both.

  

Since every element of $A$ and $B$ is in $C$ and every element of $A$ VB is also in $C$.

  

Therefore, if $A \leq C$ and $B \leq C$ then $A \cup B \leq C$

  

Let $U=\{1,2,3,4\}, A=\{1,2\}, B=\{1,2,3\}, C=\{2\}$

  

$A \cap(B \cap C)^{c}$

  

$=\{1,2\} \cap(\{2\})^{c}$

  

$=[1,2\} \cap[1,3,4]$

  

$=\{1]$

  

$A \cap(B \cap C)^{C} \neq \varnothing$ (it's not empty), the refore the statement is false

  

if $A \subseteq B$, then $P(A) \subseteq P(B)(T m r)$

  

$A \subseteq B$ : Every element in $A$ is also an element in $B$

  

$P(A)$ : Contains all subsets of $A$

  

$P(B)$ : Contains all subsets of $B$

  

Since every element in $A$ is also in $B$, every subset of $A$ is also a subset of $B$. Therefore, every element in $P(A)$ is also an element in $P(B)$ therefore if $A \subseteq B$, then $P(A) \subseteq P(B)$

  

$P(A \cup B) \subseteq P(A) \cup P(B)$ (False)

  

Let $A:[1]$ and $B=[2]$

  

$\left.P(A \cup B)=P\left(q_{1}, 2\right\}\right)=\{\phi,\{1\},\{2\},\{1,2\}\}$

  

$P(A) \cup P(B)=\{\phi,\{1]\} \cup\{\phi,[2\}]=[\phi,[1],[2]\}$

  

Therefore, $P(A \cup B) \notin P(A) \cup P(B)$

  

Commutative law

  

(b) Distributive law

  

(c)

  

Commutative law

  

Set difference law

  

Set difference law

  

Commutative law

  

(d)

  

De Morgan's law

  

Double Complement law

  

(f)

  

Distributive law

  

(g)

  

Set difference law

  

$(A \cup B)-C=(A \cup B) \cap C^{C}$

  

$=\left(A \cap C^{c}\right) \cup\left(B \cap C^{c}\right)$

  

$=(A-C) \cup(B-C)$

$(A \cap B) \cup C=(A \cup C) \cap(B \cup C)$

  

$L H S=(A \cap B) \cup C$

  

$=C \cup(A \cap B)$ commutative law

  

$=(C \cup A) \cap(C \cup B)$ distributive law

  

$=(A \cup C) \cap(B \cup C)$ commutative law

  

$A \cup(B-A)=A \cup B$

  

LHS $=A \cup(B-A)$

  

$=A \vee\left(B \cap A^{C}\right)$ set difference

  

$=(A \cup B) \cap\left(A \cup A^{C}\right)$ distributive

  

$=(A \cup B) \cap \cup$ complement lan

  

$=A \cup B \quad$ identity law

  

$(A-B) \cup(B-A)=(A \cup B)-(A \cap B)$

  

$L A S=(A-B) \cup(B-A)$

  

$=\left(A \cap B^{C}\right) \cup\left(B \cap A^{c}\right)$ set difference

  

$\left.:\left[\left(A \cap B^{c}\right) \cup B\right] \cap\left[\left(A \cap B^{c}\right) \cup A^{c}\right)\right]$ Tistributive

  

$=\left[\left(B \cup\left(A \cap B^{c}\right)\right] \cap\left[A^{c} \cup\left(A \cap B^{c}\right)\right]\right.$ Commantative law

  

$=\left[(B \cup A) \cap\left(B \cup B^{C}\right)\right] \cap\left[\left(A^{C} \cup A\right) \cap\left(A^{C} \cup B^{c}\right)\right]$ Distributive

  

$=\left[(A \cup B) \cap\left(B \cup B^{C}\right)\right] \cap\left[\left(A \cup A^{C}\right) \cap\left(A^{c} \cup B^{C}\right)\right]$ communtative law

  

$=(A \cup B) \cap\left(B \cup B^{C}\right) \cap\left(A \cup A^{C}\right) \cap\left(A \cup B^{C}\right)$ Associative law

  

$=(A \cup B) \cap \cup \cap \cup \cap\left(A \cup B^{C}\right)$ complement law

  

$:(A \cup B) \cap\left(A \cup B^{C}\right)$ complement law

  

$=(A \cup B)-(A \cap B)$ Set difference

  

$A \cap\left(\left(B \cup A^{C}\right) \cap B^{C}\right)$

  

$=A \cap\left(B \cap B^{C} \cup A^{c} \cap B^{C}\right)$ distributive

  

$=A \cap\left(\phi \cup A^{c} \cap B^{c}\right)$ complement

  

$=A \cap\left(A^{c} \cap B^{c}\right)$ identity law for union: $A \cup \emptyset=A$

  

$=\left(A \cap A^{C}\right) \cap B^{C} \quad$ associative law

  

$=\varnothing \cap B^{C}$ complement law

  

$=\varnothing \quad$ universal bound law

  

## Exercise 6.4

  

by the complement law for +

  

by the distributive law for + over.

  

by the complement law for.

a. $O=a \cdot(a, \bar{a})$ complement lau for.

  

$=(a, a) \cdot \bar{a}$ associative lav for.

  

$=a \cdot \bar{a} \quad$ complement low

  

$=0$. complement law for.

  

$\overline{0}+0=1$, which is the definition of the complement when $\overline{0}+0=1$

  

$\overline{0}+0=\dot{0}$, the identity lar for addition states that $x=0=x, 30 \overline{0}+0=\overline{0}$

  

$\overline{0}=\overline{0}$, by substituting $\overline{0}+0$ with $\overline{0}$

  

$\dot{\sigma}+0=1$, by substituting $\dot{\sigma}$ with 1 , based on definitition of complement

  

$\therefore \overline{0}=1$

  

(b) $i .1=0$, definition of complement where $i .1=0$

  

$\tau .1=i$, identity law for maltiplication

  

$T=i$, substituting $i .1$ with $i$

  

$i .1=0$, substituting $i$ with 0 , besed on defintion of complement

  

$\therefore \quad T=0$

  

$a \cdot b+(\bar{a}+\bar{b})=(\bar{a}+\bar{b})+(a \cdot b)$ connutatik lar for +

  

$=((\bar{a}+\bar{b})+a) \cdot((\bar{a}+\bar{b})+b)$ distributic lev of + over.

  

$=((\bar{b}+\bar{a})+a) \cdot(\bar{a}+(\bar{b}+b))$ compuntative and ascocssice for + $=(\bar{b}+(\bar{a}+a)) \cdot(\bar{a}+(b+\bar{b}))$ ascocstile and commutative for + $=(\bar{b}+(a+\bar{a})) \cdot(\bar{a}+1)$ commutatle and complement laws for +

  

$=(\bar{b}+1) .1$ complement and mikesal bound laws ar +

  

$=1$. 1 universal buend law Not

  

$=1$ identity law for.

a. $b+(\bar{a}+\bar{b})=1$

  

$(a \cdot b) \cdot(\bar{a}+\bar{b})=0$

  

$L H S=((a . b) \cdot \bar{a})+(((a, b) \cdot \bar{b})$ distributive law of. over +

  

$=((b \cdot a) \cdot \bar{c})+((a \cdot(b \cdot \bar{b}))$ commutative and associative laus for.

  

$=(b \cdot(a, \bar{a}))+(a, 0)$ associative and complement laws for

  

$=(b, 0)+0$ complement and eniverscl bound laws for.

  

$=0+0 \quad$ miversel bound lar for.

  

$=0$

  

identity lar for $t$.

  

$\therefore \bar{a} \cdot b=\bar{a}+\bar{b}$.

  

Not a statement, because its neither tave nor fabe

  

Is a statement, because hypothesis is not twe so whe ther what the conchrion states, its goly $t$ be the (Vacuous Truth)

  

No, because if a program lists itself, then it shouldn't be in the list, but if it doesn't list itself then it should be in the list. This creates a logical contradiction so no such program exists